<?xml version="1.0"?>

<rdf:RDF
     xmlns:cc="http://creativecommons.org/ns#"
     xmlns:rdf="http://www.w3.org/1999/02/22-rdf-syntax-ns#"
     xmlns:owl="http://www.w3.org/2002/07/owl#"
     xmlns:rico="http://www.ica.org/standards/RiC/ontology#"
     xmlns:xml="http://www.w3.org/XML/1998/namespace"
     xmlns:xsd="http://www.w3.org/2001/XMLSchema#"
     xmlns:dcterms="http://purl.org/dc/terms/"
     xmlns:skos="http://www.w3.org/2004/02/skos/core#"
     xmlns:rdfs="http://www.w3.org/2000/01/rdf-schema#"
     xmlns:rico-vocabs-1="http://www.ica.org/standards/RiC/vocabularies/recordSetTypes#"
          xmlns:dc="http://purl.org/dc/elements/1.1/">
    <owl:Ontology rdf:about="http://www.ica.org/standards/RiC/vocabularies/recordSetTypes">
       
        <dc:publisher xml:lang="en">International Council on Archives</dc:publisher>
        <skos:prefLabel>Record Set Types</skos:prefLabel>
        <dc:title xml:lang="en">International Council on Archives Records in Contexts Vocabulary for Record Set Types</dc:title>
        <dc:rights xml:lang="en">Copyright International Council on Archives (ICA),
            2018-....
            All rights reserved for this preliminary version (contact florence.clavaud@culture.gouv.fr).</dc:rights>
        <owl:versionInfo xml:lang="en">Preliminary version dated September 4th, 2018.
        This version only includes the concepts defined in ICA-ISAD(G) glossary.</owl:versionInfo>
        <dc:contributor xml:lang="en">Daniel Pitti (University of Virginia, USA), chair of EGAD</dc:contributor>
        <dc:creator xml:lang="en">International Coucil on Archives Expert Group on Archival Description (ICA EGAD)</dc:creator>
        <dc:creator xml:lang="en">Florence Clavaud (Archives nationales de France), lead of EGAD RiC-O team</dc:creator>
    </owl:Ontology>
    


    <!-- 
    ///////////////////////////////////////////////////////////////////////////////////////
    //
    // Individuals
    //
    ///////////////////////////////////////////////////////////////////////////////////////
     -->

    


    <!-- rico-vocabs-1:Collection -->

    <owl:NamedIndividual rdf:about="http://www.ica.org/standards/RiC/vocabularies/recordSetTypes#Collection">
        <rdf:type rdf:resource="http://www.w3.org/2004/02/skos/core#Concept"/>
        <skos:inScheme rdf:resource="http://www.ica.org/standards/RiC/vocabularies/recordSetTypes"/>
        <skos:definition xml:lang="en">An artificial assemblage of documents accumulated on the basis of some common
characteristic without regard to the provenance of those documents. Not to be confused
with an archival fonds.
(From ICA ISAD(G))</skos:definition>
        <skos:prefLabel xml:lang="en">collection</skos:prefLabel>
    </owl:NamedIndividual>
    


    <!-- rico-vocabs-1:File -->

    <owl:NamedIndividual rdf:about="http://www.ica.org/standards/RiC/vocabularies/recordSetTypes#File">
        <rdf:type rdf:resource="http://www.w3.org/2004/02/skos/core#Concept"/>
        <skos:inScheme rdf:resource="http://www.ica.org/standards/RiC/vocabularies/recordSetTypes"/>
        <skos:definition xml:lang="en">An organized unit of documents grouped together either for current use by the creator or
in the process of archival arrangement, because they relate to the same subject, activity, or
transaction. A file is usually the basic unit within a record series.
(From ICA ISAD(G))</skos:definition>
        <skos:prefLabel xml:lang="en">file</skos:prefLabel>
    </owl:NamedIndividual>
    


    <!-- rico-vocabs-1:Fonds -->

    <owl:NamedIndividual rdf:about="http://www.ica.org/standards/RiC/vocabularies/recordSetTypes#Fonds">
        <rdf:type rdf:resource="http://www.w3.org/2004/02/skos/core#Concept"/>
        <skos:inScheme rdf:resource="http://www.ica.org/standards/RiC/vocabularies/recordSetTypes"/>
        <skos:definition xml:lang="en">The  whole  of  the  records,  regardless  of  form  or  medium,  organically  created  and/or
accumulated  and used by a particular person, family, or corporate body in the course of that
creator&apos;s activities and functions.</skos:definition>
        <skos:prefLabel xml:lang="en">fonds</skos:prefLabel>
    </owl:NamedIndividual>
    


    <!-- rico-vocabs-1:RecordSetTypes -->

    <owl:NamedIndividual rdf:about="http://www.ica.org/standards/RiC/vocabularies/recordSetTypes">
        <rdf:type rdf:resource="http://www.w3.org/2004/02/skos/core#ConceptScheme"/>
        <skos:hasTopConcept rdf:resource="http://www.ica.org/standards/RiC/vocabularies/recordSetTypes#Collection"/>
        <skos:hasTopConcept rdf:resource="http://www.ica.org/standards/RiC/vocabularies/recordSetTypes#File"/>
        <skos:hasTopConcept rdf:resource="http://www.ica.org/standards/RiC/vocabularies/recordSetTypes#Fonds"/>
        <skos:hasTopConcept rdf:resource="http://www.ica.org/standards/RiC/vocabularies/recordSetTypes#Series"/>
    </owl:NamedIndividual>
    


    <!-- rico-vocabs-1:Series -->

    <owl:NamedIndividual rdf:about="http://www.ica.org/standards/RiC/vocabularies/recordSetTypes#Series">
        <rdf:type rdf:resource="http://www.w3.org/2004/02/skos/core#Concept"/>
        <skos:inScheme rdf:resource="http://www.ica.org/standards/RiC/vocabularies/recordSetTypes"/>
        <skos:definition xml:lang="en">Documents arranged in accordance with a filing system or maintained as a unit because
they result from the same accumulation or filing process, or the same activity; have a
particular form; or because of some other relationship arising out of their creation, receipt,
or use. A series is also known as a records series.</skos:definition>
        <skos:prefLabel xml:lang="en">series</skos:prefLabel>
    </owl:NamedIndividual>
    


    <!-- rico-vocabs-1:Sub-fonds -->

    <owl:NamedIndividual rdf:about="http://www.ica.org/standards/RiC/vocabularies/recordSetTypes#Sub-fonds">
        <rdf:type rdf:resource="http://www.w3.org/2004/02/skos/core#Concept"/>
        <skos:broader rdf:resource="http://www.ica.org/standards/RiC/vocabularies/recordSetTypes#Fonds"/>
        <skos:inScheme rdf:resource="http://www.ica.org/standards/RiC/vocabularies/recordSetTypes"/>
        <skos:definition xml:lang="en">A subdivision of a fonds containing a body of related records corresponding to
administrative subdivisions in the originating agency or organization or, when that is not
possible, to geographical, chronological, functional, or similar groupings of the material
itself. When the creating body has a complex hierarchical structure, each sub-fonds has as
many subordinate sub-fonds as are necessary to reflect the levels of the hierarchical
structure of the primary subordinate administrative unit.</skos:definition>
        <skos:prefLabel xml:lang="en">sub-fonds</skos:prefLabel>
    </owl:NamedIndividual>
</rdf:RDF>



<!-- Generated by the OWL API (version 4.2.5.20160517-0735) https://github.com/owlcs/owlapi -->

